<font face="times new roman">

* **Definition [*Big "oh"*]**: *f*(*n*) = *O*(*g*(*n*)) if and only if there exist positive constants *c* and *n*~0~ such that *f*(*n*) $\leq$ *cg*(*n*) for all *n*, *n*$\geq$ *n*~0~.
1. 3*n* + 2 = *O*(*n*)
    * *f*(*n*) = 3*n* + 2, *g*(*n*) = *n*. when *c* = 4 and *n*~0~ = 2, that 3*n* + 2 $\leq$ 4*n*, for all *n* $\geq$ 2. so 3*n* + 2 = *O*(*n*).
2. 3*n* + 3 = *O*(*n*)
    * *f*(*n*) = 3*n* + 3, *g*(*n*) = n,
when *c* = 4 and *n*~0~ = 3, that 3*n* + 3 $\leq$ 4*n*, for all *n* $\geq$ 3. so 3*n* + 3 = *O*(*n*).

</font>
