<font face="times new roman">

* **Definition [Omega]**: *f*(*n*) = $\Omega$(*g*(*n*)) iff there exist positive constants *c* and *n*~0~ such that *f*(*n*) $\geq$ *cg*(*n*) for all *n*, *n*$\geq$ *n*~0~.
1. 3*n* + 2 = $\Omega$(*n*)
    * when *c* = 3 and *n*~0~ = 1, that 3*n* + 2 $\geq$ 3*n*, for all *n* $\geq$ 1. so 3*n* + 2 = $\Omega$(*n*).
2. 10*n*^2^ + 4*n* + 2 = $\Omega$(*n*^2^)
    * when *c* = 10 and *n*~0~ = 1, that 10*n*^2^ + 4*n* + 2 $\geq$ 10*n*^2^, for all *n* $\geq$ 1 . so 10*n*^2^ + 4*n* + 2 = $\Omega$(*n*^2^)

</font>