<font face="times new roman">

* **Definition [Theta]**: *f*(*n*) = $\Theta$(*g*(*n*)) iff there exist positive constants *c*~1~,*c*~2~ and *n*~0~ such that *c*~1~ *g*(*n*)$\leq$ *f*(*n*) $\leq$ *c*~2~ *g*(*n*) for all *n*, *n*$\geq$ *n*~0~.
1. 3*n* + 2 = $\Theta$(n)
    * when *c*~1~ = 3, *c*~2~ = 4, *n*~0~ = 2, that 3*n* $\leq$ 3*n* + 2 $\leq$ 4*n*, for all *n* $\geq$ 2. so 3*n* + 2 = $\Theta$(n).
2. 10*n*^2^ + 4 *n* + 2 = $\Theta$(*n*^2^)
    * when *c*~1~ = 10, *c*~2~ = 13 ,*n*~0~ = 2, that 10*n*^2^ $\leq$ 10*n*^2^ + 4 *n* + 2 $\leq$ 13*n*^2^, for all *n* $\geq$ *n*~0~. so 10*n*^2^ + 4 *n* + 2 = $\Theta$(*n*^2^).

</font>