<font face="times new roman">

8. show that the following equalities are correct:

(a). 5*n*^2^ - 6*n* = $\Theta$(*n*^2^)

Ans: when *c*~1~ = 4, *c*~2~ = 5, and *n*~0~ = 3, that 4*n*^2^ $\leq$ 5*n*^2^ - 6*n* $\leq$ 5*n*^2^, for all *n* $\geq$ 3. so 5*n*^2^ - 6*n* = $\Theta$(*n*^2^)

(b). *n*! = *O*(*n^n^*)

Ans: when *c* = 1, *n*~0~ = 1,that *n*! = 1*n^n^*, for all *n* $\geq$ 1.so *n*! = *O*(*n^n^*)

(c). 2*n*^2^2^n^ + *n*$\log$*n* = $\Theta$(*n*^2^2^n^)

Ans: when *c*~1~ = 2,*c*~2~ = 3, and *n*~0~ = 1, that 2*n*^2^2^n^ + *n*$\log$*n* $\geq$ 2*n*^2^2^n^ and 2*n*^2^2^n^ + *n*$\log$*n* $\leq$ 3*n*^2^2^n^, for all *n* $\geq$ 1. so 2*n*^2^2^n^ + *n*$\log$*n* = $\Theta$(*n*^2^2^n^)

(d). $\sum^n_{i = 0}i^2$ = $\Theta$(*n*^3^)

Ans: $\sum^n_{i = 0}$*i* ^2^ = $\frac{n(n+1)(2n+1)}{6}$ = $\frac{2n^3+3n^2+n}{6}$. when *c*~1~ = $\frac13$, *c*~2~ = 1, and *n*~0~ = 1, that $\sum^n_{i = 0}i^2$ $\geq$ $\frac13$*n*^3^ and $\sum^n_{i = 0}i^2$ $\leq$ *n*^3^,for all *n* $\geq$ 1. so $\sum^n_{i = 0}i^2$ = $\Theta$(*n*^3^)

* note: $\sum^n_{i = 0}i^d$ =  *n* ^d+1^ <font face="標楷體">之多項式</font>

(e). $\sum^n_{i = 0}i^3$ = $\Theta$(*n*^4^)

Ans: true.

</font>
